Tutorial tidying

examples/Tutorial.v
@@ -1,15 +1,15 @@
 (** * Tutorial for QuickChick *)
 
-(** QuickChick is a clone of Haskell's QuickCheck, slightly on steroids.  This
-    tutorial explores basic aspects of random property-based testing and details
-    the majority of features of QuickChick.
-
-*)
+(** QuickChick is a clone of Haskell's QuickCheck, slightly on
+    steroids.  This tutorial explores basic aspects of random
+    property-based testing and details the majority of features of
+    QuickChick. *)
 
 (* begin hide *)
 From QuickChick Require Import QuickChick.
 Import QcDefaultNotation. Open Scope qc_scope.
 Import GenLow GenHigh.
+Set Warnings "-extraction-opaque-accessed,-extraction".
 
 Require Import List ZArith.
 Import ListNotations.
@@ -21,24 +21,23 @@ From mathcomp Require Import seq ssreflect ssrbool ssrnat eqtype.
 
 (** ** Introduction *)
      
-(** It is not uncommon during a verification effort to spend many hours
-    attempting to prove a slightly false theorem, only to result in frustration
-    when the mistake is realized and one needs to start over. Other theorem
-    provers have testing tools to quickly raise one's confidence before
-    embarking on the body of the proof; Isabelle has its own QuickCheck clone,
-    as well as Nitpick, Sledgehammer and a variety of other tools; ACL2 has gone
-    a step further using random testing to facilitate its automation. QuickChick
-    is meant to fill this void for Coq. 
+(** It is not uncommon during a verification effort to spend many
+    hours attempting to prove a slightly false theorem, only to result
+    in frustration when the mistake is realized and one needs to start
+    over. Other theorem provers have testing tools to quickly raise
+    one's confidence before embarking on the body of the proof;
+    Isabelle has its own QuickCheck clone, as well as Nitpick,
+    Sledgehammer and a variety of other tools; ACL2 has gone a step
+    further using random testing to facilitate its
+    automation. QuickChick is meant to fill this void for Coq.
 
-
-    Consider the following short function [remove] that takes a natural number
-    [x] and a list of nats [l] and proceeds to remove [x] from the list. While
-    one might be tempted to pose the question "Is there a bug in this
-    definition?", such a question has little meaning without an explicit
-    specification. Here, [removeP] requires that after removing [x] from [l],
-    the resulting list does not contain any occurences of [x].
-
- *)
+    Consider the following short function [remove] that takes a
+    natural number [x] and a list of nats [l] and proceeds to remove
+    [x] from the list. While one might be tempted to pose the question
+    "Is there a bug in this definition?", such a question has little
+    meaning without an explicit specification. Here, [removeP]
+    requires that after removing [x] from [l], the resulting list does
+    not contain any occurences of [x]. *)
 
 Fixpoint remove (x : nat) (l : list nat) : list nat :=
   match l with
@@ -49,18 +48,16 @@ Fixpoint remove (x : nat) (l : list nat) : list nat :=
 Definition removeP (x : nat) (l : list nat) := 
   (~~ (existsb (fun y => beq_nat y x) (remove x l))).
 
-(** For this simple example, it is not hard to "spot" the bug by inspection. We
-    will use QuickChick to find out what is wrong.
+(** For this simple example, it is not hard to "spot" the bug by
+    inspection. We will use QuickChick to find out what is wrong.
 
-    QuickChick provides a toplevel command [QuickChick] that receives as input
-    an executable property and attempts to falsify it.  
-
-*)
+    QuickChick provides a toplevel command [QuickChick] that receives
+    as input an executable property and attempts to falsify it. *)
 
 QuickChick removeP.
 
-(** Internally, the code is extracted to OCaml, compiled and ran to obtain the output: 
-
+(** Internally, the code is extracted to OCaml, compiled and ran to
+obtain the output:
 <<
     0
 
@@ -68,31 +65,27 @@ QuickChick removeP.
 
     Failed! After 17 tests and 12 shrinks
 >>
-    
-    The output signifies that if we use an input where [x] is [0] and [l] is the
-    two element list containing two zeros, then our property fails. Indeed, we
-    can now identify that the [then] branch of [remove] fails to make a
-    recursive call, which means that only one occurence of each element will be
-    deleted. The last line of the output states that it took 17 tests to
-    identify some fault inducing input and 12 shrinks to reduce it to a minimal
-    counterexample. 
+    The output signifies that if we use an input where [x] is [0] and
+    [l] is the two element list containing two zeros, then our
+    property fails. Indeed, we can now identify that the [then] branch
+    of [remove] fails to make a recursive call, which means that only
+    one occurence of each element will be deleted. The last line of
+    the output states that it took 17 tests to identify some fault
+    inducing input and 12 shrinks to reduce it to a minimal
+    counterexample.
 
-    Before we begin to explain exactly how QuickChick magically comes up with
-    this result, it is important to point out the first (and arguably most
-    important) limitation of this tool: it requires an *executable*
-    specification. QuickChick needs to be able to "run" a property and decide
-    whether it is true or not; a definition like [remove_spec] can't be
-    QuickChecked! 
-
-*)
+    Before we begin to explain exactly how QuickChick magically comes
+    up with this result, it is important to point out the first (and
+    arguably most important) limitation of this tool: it requires an
+    *executable* specification. QuickChick needs to be able to "run" a
+    property and decide whether it is true or not; a definition like
+    [remove_spec] can't be QuickChecked! *)
 
 Definition remove_spec :=
   forall x l, ~ In x (remove x l).
 
 (** QuickChick requires either a functional spec (like [removeP]) or a
-    decidability procedure for an inductive spec. 
-
- *)
+    decidability procedure for an inductive spec. *)
 
 (** ** Property Based Random Testing Ingredients 
 
@@ -103,35 +96,31 @@ Definition remove_spec :=
     - A generator, to produce random inputs 
     - A shrinker, to reduce counterexamples.
 
-    We will now review the latter three in order. 
-
-*)
+    We will now review the latter three in order. *)
 
 (** *** Printing 
 
-    For printing, QuickChick uses a [Show] typeclass, like Haskell. 
-
- *)
+    For printing, QuickChick uses a [Show] typeclass, like Haskell. *)
 
 Print Show.
-(**  ==> Record Show (A : Type) : Type := Build_Show { show : A -> String.string }
-*)
+(**  ==> Record Show (A : Type) : Type 
+            := Build_Show { show : A -> String.string }   *)
 
-(** The [Show] typeclass contains a single function [show] from some type [A] to
-    Coq's [string]. QuickChick provides default instances for [string]s (the
-    identity function), [nat], [bool], [Z], etc. (via extraction to appropriate
-    OCaml functions for efficiency), as well as some common compound datatypes:
-    lists, pairs and options. 
+(** The [Show] typeclass contains a single function [show] from some
+    type [A] to Coq's [string]. QuickChick provides default instances
+    for [string]s (the identity function), [nat], [bool], [Z],
+    etc. (via extraction to appropriate OCaml functions for
+    efficiency), as well as some common compound datatypes: lists,
+    pairs and options.
 
-    Writing your own show instance is easy! Let's define a simple [Color]
-    datatype.
- *)
+    Writing your own show instance is easy! Let's define a simple
+    [Color] datatype. *)
 
 Inductive Color := Red | Green | Blue | Yellow.
 
-(** After ensuring we have opened the [string] scope, we can declare an instance
-    of [Show Color] by encoding [show] as a simple pattern matching on colors.
-*)
+(** After ensuring we have opened the [string] scope, we can declare
+    an instance of [Show Color] by encoding [show] as a simple pattern
+    matching on colors. *)
 
 Require Import String. Open Scope string.
 Instance show_color : Show Color :=
@@ -147,25 +136,25 @@ Instance show_color : Show Color :=
 Eval compute in (show Green).
 (** ==> "Green" : string *)
 
-(** While writing show instances is relatively straightforward, it can get tedious. 
-    The QuickChick provides a lot of automation, which will be discussed at the end 
-    of this Tutorial. 
-*)
+(** While writing show instances is relatively straightforward, it can
+    get tedious.  The QuickChick provides a lot of automation, which
+    will be discussed at the end of this Tutorial. *)
 
 (** *** Generators *)
 
 (** **** The [G] Monad *)
 
-(** The heart of property based random testing is the random generation of
-    inputs.  In QuickChick, a generator for elements of some type [A] is a
-    monadic object with type [G A]. The monad [G] serves as an abstraction over
-    random seed plumbing. Consider writing a program that given a random seed
-    generates many integers: one needs to use the given seed to produce an
-    integer while at the same time obtain a new, altered seed to use for future
-    draws. This [State]-monad like behavior is hidden behind [G].
+(** The heart of property based random testing is the random
+    generation of inputs.  In QuickChick, a generator for elements of
+    some type [A] is a monadic object with type [G A]. The monad [G]
+    serves as an abstraction over random seed plumbing. Consider
+    writing a program that given a random seed generates many
+    integers: one needs to use the given seed to produce an integer
+    while at the same time obtain a new, altered seed to use for
+    future draws. This [State]-monad like behavior is hidden behind
+    [G].
 
-    Standard monadic functions have the [Gen] suffix.    
- *)
+    Standard monadic functions have the [Gen] suffix. *)
 
 Check bindGen.
 (** ==> bindGen : G ?A -> (?A -> G ?B) -> G ?B *) 
@@ -173,30 +162,28 @@ Check bindGen.
 Check returnGen.
 (** ==> returnGen : ?A -> G ?A *)
 
-(** For those familiar with Haskell's monadic interface, QuickChick also
-    provides variants of [liftM] (as [liftGen]) with arities 1 to 5, [sequence]
-    (as [sequenceGen]) and [foldM] (as [foldGen]).
- *)
+(** For those familiar with Haskell's monadic interface, QuickChick
+    also provides variants of [liftM] (as [liftGen]) with arities 1 to
+    5, [sequence] (as [sequenceGen]) and [foldM] (as [foldGen]). *)
 
 (** **** Primitive generators *)
 
-(** 
-    Primitive generators for booleans, natural numbers and integers are provided
-    via extraction to OCaml. They can be accessed via the [choose] combinator.
+(** Primitive generators for booleans, natural numbers and integers
+    are provided via extraction to OCaml. They can be accessed via the
+    [choose] combinator.
  *)
 
 Check choose.
 (** ==> choose : Z * Z -> G Z *)
 
-(** While here [choose] is monomorphised to [Z], it actually takes an interval
-    of any type [A] that satisfies a [ChoosableFromInterval] typeclass (with
-    default standard numeric instances) and produces an object of type [A]
-    within that interval. 
+(** While here [choose] is monomorphised to [Z], it actually takes an
+    interval of any type [A] that satisfies a [ChoosableFromInterval]
+    typeclass (with default standard numeric instances) and produces
+    an object of type [A] within that interval.
 
-    We can see that in action using [Sample]. This is another toplevel command
-    by QuickChick that runs a generator a number of times and prints whatever 
-    was generated in the form of a list 
- *)
+    We can see that in action using [Sample]. This is another toplevel
+    command by QuickChick that runs a generator a number of times and
+    prints whatever was generated in the form of a list. *)
 
 Sample (choose(0, 10)).
 (** ==> [ 1, 2, 1, 9, 8, 1, 3, 6, 2, 1, 8, 0, 1, 1, 3, 5, 4, 10, 4, 6 ] *)
@@ -204,17 +191,15 @@ Sample (choose(0, 10)).
 
 (** **** Lists *)
 
-(** Due to being the most commonly used compound datatype, lists have special
-    combinators in Haskell's QuickCheck. The same is true in QuickChick; there
-    are two combinators, [listOf] and [vectorOf]. 
- *)
+(** Due to being the most commonly used compound datatype, lists have
+    special combinators in Haskell's QuickCheck. The same is true in
+    QuickChick; there are two combinators, [listOf] and [vectorOf]. *)
 
 Check listOf.
 (** ==> listOf : G ?A -> G (list ?A) *)
 
 (** [listOf] takes as input a generator for elements of type [A] and returns a
-    generator for lists of the same type.
- *)
+    generator for lists of the same type. *)
 
 Sample (listOf (choose (0,4))).
 (** ==> [ [ 0, 3, 2, 0 ], 
@@ -240,50 +225,49 @@ Sample (listOf (choose (0,4))).
        ]
 *)
 
-(** The second combinator, [vectorOf], receives an additional numeric argument
-    [n], the length of the list to be generated. 
- *)
+(** The second combinator, [vectorOf], receives an additional numeric
+    argument [n], the length of the list to be generated. *)
 
 Check vectorOf.
 (** ==> vectorOf : nat -> G ?A -> G (list ?A) *)
 
-(** This raises a question: how does [listOf] decide how big of a list to
-    generate? The answer is hidden inside the [G] monad. 
+(** This raises a question: how does [listOf] decide how big of a list
+    to generate? The answer is hidden inside the [G] monad.
   
-    In addition to handling random seed plumbing, the [G] monad also provides a
-    [Reader]-like environment with size information: a natural number [n] that
-    nominally serves as the upper bound on the depth of the generated objects.
-    QuickChick progressively tries larger and larger values for [n], in order to
-    explore larger and deeper part of the search space. Note that each generator
-    can choose to interpret this input size however it wants and there is no
-    guarantee that all generators comply to this standard - it is more of a
-    "good practice" when writing one to respect this bound. 
- *)
+    In addition to handling random seed plumbing, the [G] monad also
+    provides a [Reader]-like environment with size information: a
+    natural number [n] that nominally serves as the upper bound on the
+    depth of the generated objects.  QuickChick progressively tries
+    larger and larger values for [n], in order to explore larger and
+    deeper part of the search space. Note that each generator can
+    choose to interpret this input size however it wants and there is
+    no guarantee that all generators comply to this standard - it is
+    more of a "good practice" when writing one to respect this
+    bound. *)
 
 (** **** Custom Datatypes *)
 
 (** Naturally, a lot of the time one needs to write generators involving
     user-defined datatypes. Let's revisit our color datatype; to generate a
     color, we only need to pick one of its four constructors, [Red], [Green],
-    [Blue] and [Yellow]. This is done using [elements].
-
-*)
+    [Blue] and [Yellow]. This is done using [elements]. *)
 
 Check elements.
 (** ==> elements : ?A -> list ?A -> G ?A *)
 
-(** This is the first place where the totality checker of Coq raises a design
-    question. While Haskell's QuickCheck can simply fail raising an [error]
-    whenever the input list is empty, Coq does not allow that behavior. Instead
-    of increasing the burden to the user by requiring a proof that the list is
-    not empty or by making the return type an option, QuickChick requires an
-    additional element of type [A] as input to serve as a "default" object.  If
-    the list is not empty, [elements] returns a generator that picks an element
-    of that list; otherwise the generator always returns the default object.
+(** This is the first place where the totality checker of Coq raises a
+    design question. While Haskell's QuickCheck can simply fail
+    raising an [error] whenever the input list is empty, Coq does not
+    allow that behavior. Instead of increasing the burden to the user
+    by requiring a proof that the list is not empty or by making the
+    return type an option, QuickChick requires an additional element
+    of type [A] as input to serve as a "default" object.  If the list
+    is not empty, [elements] returns a generator that picks an element
+    of that list; otherwise the generator always returns the default
+    object.
 
-    Moreover, QuickChick provides convenient notation to hide this default if 
-    it is apparent from the structure. 
- *)
+    Moreover, QuickChick provides convenient notation to hide this
+    default if it is apparent from the structure. *)
 
 (*
 Notation            Scope     
@@ -302,7 +286,8 @@ Notation            Scope
                       (default interpretation)
 *)
 
-(** Armed with [elems], we can write the following simple [Color] generator. *)
+(** Armed with [elems], we can write the following simple [Color]
+    generator. *)
 
 Definition genColor : G Color :=
   elems [ Red ; Green ; Blue ; Yellow ].
@@ -311,12 +296,12 @@ Sample genColor.
 (** ==> [ Blue, Red, Yellow, Red, Blue, Yellow, Yellow, Blue, Green, Red, Green,
          Blue, Blue, Red, Yellow, Blue, Red, Blue, Blue, Red ] *)
 
-(** For more complicated ADTs, QuickChick provides more combinators. We will 
-    showcase them using everyone's favorite datatype: Trees! 
+(** For more complicated ADTs, QuickChick provides more
+    combinators. We will showcase them using everyone's favorite
+    datatype: Trees!
 
-    Our trees are standard binary trees; either [Leaf]s or [Node]s containing 
-    some payload of type [A] and two subtrees. 
-*)
+    Our trees are standard binary trees; either [Leaf]s or [Node]s
+    containing some payload of type [A] and two subtrees. *)
 
 Inductive Tree A :=
 | Leaf : Tree A
@@ -325,11 +310,10 @@ Inductive Tree A :=
 Arguments Leaf {A}.
 Arguments Node {A} _ _ _.
 
-(** Before getting to generators for trees, we give a simple [Show] instance. 
-    The rather inconvenient need for a local [let fix] declaration stems from
-    the fact that Coq's typeclasses (unlike Haskell's) are not automatically 
-    recursive. 
-*) 
+(** Before getting to generators for trees, we give a simple [Show]
+    instance.  The rather inconvenient need for a local [let fix]
+    declaration stems from the fact that Coq's typeclasses (unlike
+    Haskell's) are not automatically recursive. *) 
 
 Instance showTree {A} `{_ : Show A} : Show (Tree A) :=
   {| show := 
@@ -341,40 +325,40 @@ Instance showTree {A} `{_ : Show A} : Show (Tree A) :=
        in aux
   |}.
 
-(** The first combinator that actually combines different generators is [oneof]. *)
+(** The first combinator that actually combines different generators
+    is [oneof]. *)
 
 Check oneof.
 (** ==> oneof : G ?A -> list (G ?A) -> G ?A *)
 
-(** [oneof] takes a default generator and a list of generators, and picks one of
-    the generators from the list uniformly at random, as long as the list is not
-    empty.  Just like before, QuickChick introduces the notation [oneOf] to hide
-    this default element. 
+(** [oneof] takes a default generator and a list of generators, and
+    picks one of the generators from the list uniformly at random, as
+    long as the list is not empty.  Just like before, QuickChick
+    introduces the notation [oneOf] to hide this default element.
 
-    At this point, Coq's termination checker saves us from shooting ourselves in
-    the foot. The "obvious" first generator that one might write is the
-    following [genTree]: either generate a [Leaf] or a [Node] whose subtrees are 
-    generated recursively and whose payload is produced by a generator for 
-    elements of type [A].
-
-*)
+    At this point, Coq's termination checker saves us from shooting
+    ourselves in the foot. The "obvious" first generator that one
+    might write is the following [genTree]: either generate a [Leaf]
+    or a [Node] whose subtrees are generated recursively and whose
+    payload is produced by a generator for elements of type [A].*)
 
 (*
 Fixpoint genTree {A} (g : G A) : G (Tree A) :=
   oneOf [ returnGen Leaf ;
-          liftGen3 Node  g (genTree g) (genTree g) ].
-*)
+          liftGen3 Node  g (genTree g) (genTree g) ].*)
 
-(** Of course, this fixpoint will not pass Coq's termination check. Attempting
-    to justify this fixpoint to oneself, one might say that at some point the
-    random generation will pick a [Leaf] so it will eventually terminate. Sadly, 
-    in this case the expected size of the generated Tree is infinite...
+(** Of course, this fixpoint will not pass Coq's termination
+    check. Attempting to justify this fixpoint to oneself, one might
+    say that at some point the random generation will pick a [Leaf] so
+    it will eventually terminate. Sadly, in this case the expected
+    size of the generated Tree is infinite...
 
-    The solution is the standard "fuel" solution Coq users are so familiar with:
-    we add an additional natural number [sz] as a parameter; when that parameter
-    is [O] we only generate non-recursive branches, while we decrease this size
-    in each recursive call. Thus, [sz] serves as a bound on the depth of the
-    tree. 
+    The solution is the standard "fuel" solution Coq users are so
+    familiar with: we add an additional natural number [sz] as a
+    parameter; when that parameter is [O] we only generate
+    non-recursive branches, while we decrease this size in each
+    recursive call. Thus, [sz] serves as a bound on the depth of the
+    tree.
 
  *)
 
@@ -409,20 +393,21 @@ Sample (genTreeSized 3 (choose(0,3))).
          Leaf ]
 *)
 
-(** While this generator succesfully generated trees, just by observing [Sample]
-    above there is a problem: [genTreeSized] produces way too many [Leaf]s! That
-    is to be expected, 50% of the time we generate a [Leaf]. The solution is to
-    skew the distribution towards [Node]s, using the most expressive QuickChick
-    combinator, [frequency] and its associated default-lifting notation [freq].
+(** While this generator succesfully generated trees, just by
+    observing [Sample] above there is a problem: [genTreeSized]
+    produces way too many [Leaf]s! That is to be expected, 50% of the
+    time we generate a [Leaf]. The solution is to skew the
+    distribution towards [Node]s, using the most expressive QuickChick
+    combinator, [frequency] and its associated default-lifting
+    notation [freq].
  *)
 Check frequency.
 (** ==> frequency : G ?A -> seq (nat * G ?A) -> G ?A *)
 
-(** [freq] takes a list of generators, each one tagged with a natural number
-    that serves as the weight of that generator. In the following example, a
-    [Leaf] will be generated 1 / (sz + 1) of the time, while a [Node] the
-    remaining sz / (sz + 1) of the time.
-*)
+(** [freq] takes a list of generators, each one tagged with a natural
+    number that serves as the weight of that generator. In the
+    following example, a [Leaf] will be generated 1 / (sz + 1) of the
+    time, while a [Node] the remaining sz / (sz + 1) of the time.*)
 
 Fixpoint genTreeSized' {A} (sz : nat) (g : G A) : G (Tree A) :=
   match sz with
@@ -455,9 +440,8 @@ Sample (genTreeSized' 3 (choose(0,3))).
          Leaf ]
  *)
 
-(** To show case this generator, we will use the notion of mirroring a tree: swapping 
-    its left and right subtrees recursively. 
-*)
+(** To showcase this generator, we will use the notion of mirroring a
+    tree: swapping its left and right subtrees recursively. *)
    
 Fixpoint mirror {A : Type} (t : Tree A) : Tree A :=
   match t with
@@ -474,21 +458,22 @@ Fixpoint eq_tree (t1 t2 : Tree nat) : bool :=
     | _, _ => false
   end.
 
-(** One expects that [mirror] should be unipotent; mirroring a tree twice yields 
-    the original tree.  
-*)
+(** One expects that [mirror] should be unipotent; mirroring a tree
+    twice yields the original tree.  *)
+
 Definition mirrorP (t : Tree nat) := eq_tree (mirror (mirror t)) t.
 
-(** To test this assumption, we can use the [forAll] property combinator that
-    receives a generator [g] for elements of type [A] and an executable property
-    with argument [A] and tests the property on random inputs of [g]. 
- *)
+(** To test this assumption, we can use the [forAll] property
+    combinator that receives a generator [g] for elements of type [A]
+    and an executable property with argument [A] and tests the
+    property on random inputs of [g]. *)
+
 QuickChick (forAll (genTreeSized' 5 (choose (0,5))) mirrorP).
 
-(** QuickChick quickly responds that this property passed 10000 tests, so we 
-    gain some confidence in its truth. But what would happend if we had the 
-    *wrong* property? 
-*)
+(** QuickChick quickly responds that this property passed 10000 tests,
+    so we gain some confidence in its truth. But what would happend if
+    we had the *wrong* property? *)
+
 Definition faultyMirrorP (t : Tree nat) := eq_tree (mirror t) t.
 
 QuickChick (forAll (genTreeSized' 5 (choose (0,5))) faultyMirrorP).
@@ -503,24 +488,23 @@ QuickChick (forAll (genTreeSized' 5 (choose (0,5))) faultyMirrorP).
 (** The bug is found immediately and reported. However, is this counterexample
     really helpful? What is the important part of it? The reported bug is too
     big and noisy to identify the root cause of the problem. That is where
-    shrinking comes in. 
-
-*)
+    shrinking comes in. *)
 
 (** **** Shrinking *)
 
-(** Shrinking, also known as delta debugging, is a greedy process by which we
-    can find a smaller counterexample given a relatively large one. Given a
-    shrinking function [s] of type [A -> list A] and a counterexample [x] of
-    type [A] that is known to falsify some property [p], QuickChick (lazily)
-    tries [p] on all members of [s x] until it finds another counterexample;
-    then it repeats this process.
+(** Shrinking, also known as delta debugging, is a greedy process by
+    which we can find a smaller counterexample given a relatively
+    large one. Given a shrinking function [s] of type [A -> list A]
+    and a counterexample [x] of type [A] that is known to falsify some
+    property [p], QuickChick (lazily) tries [p] on all members of [s
+    x] until it finds another counterexample; then it repeats this
+    process.
 
-    This greedy algorithm can only work if all elements of [s x] are strictly 
-    "smaller" that [x] for all [x]. Most of the time, a shrinking function for 
-    some type only returns elements that are "one step" smaller. For example,  
-    consider the default shrinking function for lists provided by QuickChick. 
-*)
+    This greedy algorithm can only work if all elements of [s x] are
+    strictly "smaller" that [x] for all [x]. Most of the time, a
+    shrinking function for some type only returns elements that are
+    "one step" smaller. For example, consider the default shrinking
+    function for lists provided by QuickChick. *)
 
 Print shrinkList.
 (** ==> shrinkList = 
@@ -535,17 +519,15 @@ Print shrinkList.
           : forall A : Type, (A -> seq A) -> seq A -> seq (seq A)
 *)
 
-(** An empty list can not be shrunk - there is no smaller list. 
-    A cons cell can be shrunk in three ways: by returning the tail of the list,
-    by shrinking the tail of the list and consing the head, or by shrinking the 
-    head and consing its tail. By induction, this process can generate all smaller
-    lists.
+(** An empty list can not be shrunk - there is no smaller list.  A
+    cons cell can be shrunk in three ways: by returning the tail of
+    the list, by shrinking the tail of the list and consing the head,
+    or by shrinking the head and consing its tail. By induction, this
+    process can generate all smaller lists.
 
-    Writing a shrinking instance for trees is equally straightforward: we don't
-    shrink [Leaf]s while for [Node]s we can return the left or right subtrees,
-    shrink the payload or one of the subtrees.
-
-*)
+    Writing a shrinking instance for trees is equally straightforward:
+    we don't shrink [Leaf]s while for [Node]s we can return the left
+    or right subtrees, shrink the payload or one of the subtrees.*)
 
 Open Scope list.
 Fixpoint shrinkTree {A} (s : A -> list A) (t : Tree A) : seq (Tree A) :=
@@ -557,8 +539,8 @@ Fixpoint shrinkTree {A} (s : A -> list A) (t : Tree A) : seq (Tree A) :=
                     map (fun r' => Node x l r') (shrinkTree s r)
   end.
 
-(** Armed with [shrinkTree], we use the [forAllShrink] property combinator that 
-    takes an additional argument, a shrinker *)
+(** Armed with [shrinkTree], we use the [forAllShrink] property
+    combinator that takes an additional argument, a shrinker *)
 
 QuickChick (forAllShrink (genTreeSized' 5 (choose (0,5))) (shrinkTree shrink) faultyMirrorP).
 
@@ -566,32 +548,30 @@ QuickChick (forAllShrink (genTreeSized' 5 (choose (0,5))) (shrinkTree shrink) fa
 
 *** Failed! After 1 tests and 8 shrinks *)
 
-(** We now got a much simpler counterexample (in fact, this is one of the two
-    minimal ones) and can tell that the real problem occurs when the subtrees of 
-    a [Node] are different.
- *)
+(** We now got a much simpler counterexample (in fact, this is one of
+    the two minimal ones) and can tell that the real problem occurs
+    when the subtrees of a [Node] are different. *)
 
 (** **** Putting it all Together *)
 
-(** QuickChick, just like QuickCheck, provides an [Arbitrary] typeclass
-    parameterized over some type [A] with two objects: [arbitrary] and
-    [shrink]. 
+(** QuickChick, just like QuickCheck, provides an [Arbitrary]
+    typeclass parameterized over some type [A] with two objects:
+    [arbitrary] and [shrink].
 
-    The [arbitrary] object is a generator for elements of type [A]. If we were
-    to encode an [Arbitrary] instance for trees we would like to use
-    [genTreeSized']; however that generator takes an additional size argument. 
-    The [G] monad will provide that argument through the combinator [sized].
-
-*)
+    The [arbitrary] object is a generator for elements of type [A]. If
+    we were to encode an [Arbitrary] instance for trees we would like
+    to use [genTreeSized']; however that generator takes an additional
+    size argument.  The [G] monad will provide that argument through
+    the combinator [sized].*)
     
 Check sized.
 (** ==> sized : (nat -> G ?A) -> G ?A *)
 
-(** [sized] receives a function that given a number produces a generator, just
-    like [genTreeSized'], and returns a generator that uses the size information inside the [G] monad.
+(** [sized] receives a function that given a number produces a
+    generator, just like [genTreeSized'], and returns a generator that
+    uses the size information inside the [G] monad.
 
-    The [shrink] function is simply a shrinker like [shrinkTree]. 
-*)
+    The [shrink] function is simply a shrinker like [shrinkTree]. *)
 
 Instance genTree {A} `{Gen A} : GenSized (Tree A) := 
   {| arbitrarySized n := genTreeSized n arbitrary |}.
@@ -600,39 +580,39 @@ Instance shrTree {A} `{Shrink A} : Shrink (Tree A) :=
   {| shrink x := shrinkTree shrink x |}.
 
 (** With this [Arbitrary] instance we can once again use the toplevel
-    [QuickChick] command with just the property.  
-
-*)
+    [QuickChick] command with just the property.  *)
 
 QuickChick faultyMirrorP.
 
-(** [QuickChick] internally calls the function [quickCheck] with type [forall
-    prop. Checkable prop => prop -> Result]. But what _is_ [Checkable]? It is
-    easy to see how a boolean is [Checkable]; we can always tell if it is true
-    or not and then return a [Result], [Success]/[Failure] as appropriate.
+(** [QuickChick] internally calls the function [quickCheck] with type
+    [forall prop. Checkable prop => prop -> Result]. But what _is_
+    [Checkable]? It is easy to see how a boolean is [Checkable]; we
+    can always tell if it is true or not and then return a [Result],
+    [Success]/[Failure] as appropriate.
     
-    To see how executable properties are [Checkable], consider a single argument
-    function [p : A -> Bool] that returns a boolean. If we know that [A] has
-    [Show] and [Arbitrary] instances, we can just call [forAllShrink] with
-    [arbitrary] and [shrink]. Going a step further, the result type doesn't
-    really need to be [Bool], it can be a [Checkable]! Thus, we can provide a
-    [Checkable] instance for arbitrary functions.
-
-*)
+    To see how executable properties are [Checkable], consider a
+    single argument function [p : A -> Bool] that returns a
+    boolean. If we know that [A] has [Show] and [Arbitrary] instances,
+    we can just call [forAllShrink] with [arbitrary] and
+    [shrink]. Going a step further, the result type doesn't really
+    need to be [Bool], it can be a [Checkable]! Thus, we can provide a
+    [Checkable] instance for arbitrary functions.*)
 
 Print testFun.
 
 (** **** Collecting Statistics *)
 
-(** Earlier in this tutorial we claimed that [genTreeSized] produced "too many"
-    [Leaf]s. But how can we justify that? Just looking at the result of [Sample]
-    gives us an idea that something is going wrong but just observing a handful
-    of samples cannot realistically provide statistical guarantees. That is
-    where [collect], another property combinator, comes in. In Haskell notation,
-    [collect] would have the type [collect : Show A, Checkable prop => A -> prop
-    -> prop]; it takes some value of type [A] that can be shown and a property,
-    and returns the property itselft. Whenever the resulting property is
-    exercised, the [A] object is captured and statistics are collected. 
+(** Earlier in this tutorial we claimed that [genTreeSized] produced
+    "too many" [Leaf]s. But how can we justify that? Just looking at
+    the result of [Sample] gives us an idea that something is going
+    wrong but just observing a handful of samples cannot realistically
+    provide statistical guarantees. That is where [collect], another
+    property combinator, comes in. In Haskell notation, [collect]
+    would have the type [collect : Show A, Checkable prop => A -> prop
+    -> prop]; it takes some value of type [A] that can be shown and a
+    property, and returns the property itselft. Whenever the resulting
+    property is exercised, the [A] object is captured and statistics
+    are collected.
 
     For example, consider a [size] function on [Tree]s.
  *)
@@ -643,9 +623,9 @@ Fixpoint size {A} (t : Tree A) : nat :=
     | Node _ l r => 1 + size l + size r
   end.
 
-(** If we were to write a dummy property to check our generators and measure the
-    size of generated trees, we could use [treeProp] below. 
-*)
+(** If we were to write a dummy property to check our generators and
+    measure the size of generated trees, we could use [treeProp]
+    below. *)
 
 Definition treeProp (g : nat -> G nat -> G (Tree nat)) n :=
   forAll (g n (choose (0,n))) (fun t => 
@@ -714,17 +694,16 @@ QuickChick (treeProp genTreeSized' 5).
 2 : 27
 +++ OK, passed 10000 tests
 
-A lot fewer terms have small sizes, allowing us to explore larger terms
-*)
+A lot fewer terms have small sizes, allowing us to explore larger terms*)
 
 (** ** Avoiding Work  :) *)
 
-(** While a lot of time putting a bit of time and effort in a generator and a
-shrinker, the examples shown here are fairly straightforward. After writing a
-couple of [Show] and [Arbitrary] instances, it can get tedious and boring. That
-is precisely why [QuickChick] provides some automation in deriving such instances for _plain_ datatypes automatically. 
-
-*)
+(** While a lot of time putting a bit of time and effort in a
+    generator and a shrinker, the examples shown here are fairly
+    straightforward. After writing a couple of [Show] and [Arbitrary]
+    instances, it can get tedious and boring. That is precisely why
+    [QuickChick] provides some automation in deriving such instances
+    for _plain_ datatypes automatically. *)
 
 Derive Arbitrary for Tree.
 (* genSTree is defined *)
